src/Values.v
@@ -1,10 +1,11 @@
 Require Import AST.
 Require Import String.
 Require Import Coqlib.
+Require Import Bitvectors.
 
 Inductive val :=
 | bit (b : bool) (* Can we ever get this now? *)
-| bits {n} (b : BitV n) (* bitvector *)
+(*| bits {n} (b : BitV n) (* bitvector *)*)
 | close (id : ident) (e : Expr) (E : ident -> option val)  (* closure *)
 | tclose (id : ident) (e : Expr) (E : ident -> option val) (* type closure *)
 | tuple (l : list val) (* heterogeneous tuples *)
@@ -13,19 +14,69 @@ Inductive val :=
 | vcons (v : val) (e : Expr) (E : ident -> option val) (* lazy list: first val computed, rest is thunked *)
 | vnil (* empty list *)
 .
-(*
-| vcomp (e : Expr) (E : ident -> option val) (l : list (list Match)) (* lazy list comprehension *)
-| vapp (l1 l2 : Expr) (E : ident -> option val)
-| vsplit (n m : Z) (l : Expr) (E : ident -> option val)
-(*| vsplitAt (t1 t2 t3 : Typ) (l : Expr) (E : ident -> option val)*)
-(* a slice of an underlying list *)
-(* NOTE: indexing into slices can be a bit wonky *)
-(* you can slice l from 3 to 6 *)
-(* then, access 1 would actually go to element 4 of l *)
-(* only then would you do any computation on the lazy list *)
-| vslice (l h : nat) (e : Expr) (E : ident -> option val)
-.
- *)
+
+(* convert a forced list of bits to a bitvector *)
+Fixpoint to_bitv {ws : nat} (l : list val) : option (BitV ws) :=
+  match l, ws with
+  | nil, O => Some (@repr 0 0)
+  | (bit b) :: r, S n =>
+    match @to_bitv n r with
+    | Some bv => Some (@repr (S n) (unsigned bv + if b then (two_power_nat (S n)) else 0))
+    | None => None
+    end
+  | _,_ => None
+  end.
+
+Fixpoint from_bitv' {ws : nat} (n : nat) (bv : BitV ws) : list val :=
+  match n with
+  | O => nil
+  | S n' => (bit (testbit bv (Z.of_nat n')) :: from_bitv' n' bv)
+  end.
+
+Definition from_bitv {ws : nat} (bv : BitV ws) : list val :=
+  from_bitv' ws bv.
+
+Lemma tobit_length :
+  forall l ws bv,
+    @to_bitv ws l = Some bv ->
+    ws = length l.
+Proof.
+  induction l; intros.
+  unfold to_bitv in *. destruct ws; simpl in H; inv H. reflexivity.
+  destruct ws; simpl in H. destruct a; simpl in H; inv H.
+  destruct a; simpl in H; try solve [inv H].
+  match goal with
+  | [ H : context[ match ?X with _ => _ end ] |- _ ] => destruct X eqn:?
+  end; inv H.
+  eapply IHl in Heqo. simpl. auto.
+Qed.
+  
+(* @NATE: This lemma, or something like it, is what we want proven about to_bitv and from_bitv *)
+Lemma tobit_frombit :
+  forall l ws bv,
+    to_bitv l = Some bv ->
+    @from_bitv' ws ws bv = l.
+Proof.
+  induction l; intros.
+  eapply tobit_length in H. subst. simpl. reflexivity.
+  destruct ws. simpl in H. destruct a; congruence.
+  simpl. 
+  simpl in H. destruct a; try congruence.
+  match goal with
+  | [ H : context[ match ?X with _ => _ end ] |- _ ] => destruct X eqn:?
+  end; inv H.
+  eapply IHl in Heqo.
+  f_equal. f_equal.
+Admitted.
+
 
 Definition env := ident -> option val.
 Definition empty : env := fun _ => None.
+
+(* Conversion from fully computed finite list to lazy list via trivial thunking *)
+Fixpoint thunk_list (l : list val) : val :=
+  match l with
+  | nil => vnil
+  | f :: r =>
+    vcons f (EVar (0,""%string)) (extend empty (0,""%string) (thunk_list r))
+  end.
