src/Semantics.v
@@ -39,13 +39,6 @@ Fixpoint bind_decl_groups (lg : list DeclGroup) (ge : genv) : genv :=
     bind_decl_groups gs (bind_decl_group g ge)
   end.
 
-(* Conversion from fully computed finite list to lazy list via trivial thunking *)
-Fixpoint thunk_list (l : list val) : val :=
-  match l with
-  | nil => vnil
-  | f :: r =>
-    vcons f (EVar (0,""%string)) (extend empty (0,""%string) (thunk_list r))
-  end.
 
 (* record lookup *)
 Fixpoint lookup (str : string) (l : list (string * val)) : option val :=
@@ -57,9 +50,8 @@ Fixpoint lookup (str : string) (l : list (string * val)) : option val :=
 
 Inductive eval_expr (ge : genv) : env -> Expr -> val -> Prop :=
 | eval_builtin_sem :
-    forall E l vs b v,
-      Forall2 (eval_expr ge E) l vs ->
-      eval_builtin ge b vs v ->
+    forall E l b v,
+      eval_builtin ge E b l v ->
       eval_expr ge E (EBuiltin b l) v
 | eval_list :
     forall E l vs vres,
@@ -89,7 +81,6 @@ Inductive eval_expr (ge : genv) : env -> Expr -> val -> Prop :=
       eval_expr ge E c (bit b) ->
       eval_expr ge E (if b then t else f) v ->
       eval_expr ge E (EIf c t f) v
-                
 | eval_local_var :
     forall E id v,
       E id = Some v ->
@@ -113,11 +104,11 @@ Inductive eval_expr (ge : genv) : env -> Expr -> val -> Prop :=
     forall E exp decls v, 
       eval_expr (bind_decl_groups decls ge) E exp v ->
       eval_expr ge E (EWhere exp decls) v
-| eval_list_sel :
-    forall E idx {w : nat} (i : BitV w) v e,
-      eval_expr ge E idx (bits i) ->
-      select_list ge E (Z.to_nat (unsigned i)) e v ->
-      eval_expr ge E (ESel e (ListSel idx)) v
+(* | eval_list_sel : *)
+(*     forall E idx {w : nat} (i : BitV w) v e, *)
+(*       eval_expr ge E idx (bits i) -> *)
+(*       select_list ge E (Z.to_nat (unsigned i)) e v -> *)
+(*       eval_expr ge E (ESel e (ListSel idx)) v *)
 | eval_tapp :
     forall E e id e' E' v t,
       eval_expr ge E e (tclose id e' E') ->
@@ -126,10 +117,44 @@ Inductive eval_expr (ge : genv) : env -> Expr -> val -> Prop :=
 | eval_tabs :
     forall E e id,
       eval_expr ge E (ETAbs id e) (tclose id e E)
-(* TODO: fix this *)
-(*| eval_comp :
-    forall E e l,
-      eval_expr ge E (EComp e l) (vcomp e E l)*)
+| eval_append_nil :
+    forall E e1 e2 v,
+      eval_expr ge E e1 vnil ->
+      eval_expr ge E e2 v ->
+      eval_expr ge E (EAppend e1 e2) v
+| eval_append_cons :
+    forall v eR ER E  vfirst vrest E' e1 e2,
+      eval_expr ge E e1 (vcons v eR ER) ->
+      eval_expr ge ER eR vfirst ->
+      eval_expr ge E e2 vrest ->
+      E' = extend (extend empty (1,"first") vfirst) (0,"rest") vrest ->
+      eval_expr ge E (EAppend e1 e2) (vcons v (EAppend (EVar (1,"first")) (EVar (0,"rest"))) E')
+| eval_head :
+    forall E e v e' E',
+      eval_expr ge E e (vcons v e' E') ->
+      eval_expr ge E (EHead e) v
+| eval_tail_zero :
+    forall E e v e' E',
+      eval_expr ge E e (vcons v e' E') ->
+      eval_expr ge E (ETail O e) v
+| eval_tail_succ :
+    forall E e v e' E' n v',
+      eval_expr ge E e (vcons v e' E') ->
+      eval_expr ge E' (ETail n e') v' ->
+      eval_expr ge E (ETail (S n) e) v'
+
+(* Force complete evaluation of a lazy list *)
+(* Used for converting a list of bits into a number to evaluate arithmetic *)
+with force_list (ge : genv) : env -> Expr -> list val -> Prop :=
+     | force_nil :
+         forall E e,
+           eval_expr ge E e vnil ->
+           force_list ge E e nil
+     | force_cons :
+         forall E e e' E' l v,
+           eval_expr ge E e (vcons v e' E') ->
+           force_list ge E' e' l ->
+           force_list ge E e (v::l)
                 
 (* select the nth element from a lazy list *)
 with select_list (ge : genv) : env -> nat -> Expr -> val -> Prop :=
@@ -202,7 +227,6 @@ with index_match (ge : genv) : env -> nat -> list Match -> env -> Prop :=
            index_match ge E n r E' ->
            select_list ge E O e v ->
            index_match ge E n ((From id e) :: r) (extend E' id v)
-(* because the lists are potentially infinite, we can't  *)
 with matchlength (ge : genv) : env -> list Match -> nat -> Prop :=
      | len_one :
          forall E id e n,
@@ -224,129 +248,135 @@ with length (ge : genv) : env -> Expr -> nat -> Prop :=
            eval_expr ge E e (vcons v re rE) ->
            length ge rE re n ->
            length ge E e (S n)
-with eval_builtin (ge : genv) : builtin -> list val -> val -> Prop :=
-| eval_demote :
-    forall {ws : nat} (w n : Z) (b : BitV ws),
-      ws = Z.to_nat w ->
-      b = @repr ws n ->
-      eval_builtin ge Demote ((typ (TCon (TC (TCNum n)) nil)) :: (typ (TCon (TC (TCNum w)) nil)) :: nil) (bits b)
+with eval_builtin (ge : genv) : env -> builtin -> list Expr -> val -> Prop :=
+(* | eval_demote : *)
+(*     forall {ws : nat} (w n : Z) (b : BitV ws), *)
+(*       ws = Z.to_nat w -> *)
+(*       b = @repr ws n -> *)
+(*       eval_builtin ge Demote ((typ (TCon (TC (TCNum n)) nil)) :: (typ (TCon (TC (TCNum w)) nil)) :: nil) (bits b) *)
 | eval_plus :
-    forall {w : nat} (b1 b2 b3 : BitV w) t,
-      b3 = @add w b1 b2 ->
-      eval_builtin ge Plus (t :: (bits b1) :: (bits b2) :: nil) (bits b3)
-| eval_minus :
-    forall {w : nat} (b1 b2 b3 : BitV w) t,
-      b3 = @sub w b1 b2 ->
-      eval_builtin ge Minus (t :: (bits b1) :: (bits b2) :: nil) (bits b3)
-| eval_times :
-    forall {w : nat} (b1 b2 b3 : BitV w) t,
-      b3 = @mul w b1 b2 ->
-      eval_builtin ge Times (t :: (bits b1) :: (bits b2) :: nil) (bits b3)
-| eval_div :
-    forall {w : nat} (b1 b2 b3 : BitV w) t,
-      b3 = @divu w b1 b2 -> (* I assume that division is unsigned in cryptol *)
-      unsigned b2 <> 0 -> (* no division by 0 *)
-      eval_builtin ge Div (t :: (bits b1) :: (bits b2) :: nil) (bits b3)
-| eval_mod :
-    forall {w : nat} (b1 b2 b3 : BitV w) t,
-      b3 = @modu w b1 b2 ->
-      eval_builtin ge Mod (t :: (bits b1) :: (bits b2) :: nil) (bits b3)
-(* | eval_exp : *) (* TODO: write pow over bits, or implement in Cryptol *)
-(*     forall {w : nat} {nz : w <> O} (b1 b2 b3 : BitV w) t, *)
-(*       b3 = @exp w nz b1 b2 -> *)
-(*       eval_builtin ge Exp (t :: (bits b1) :: (bits b2) :: nil) (bits b3) *)
-(* | eval_lg2 : *) (* TODO: what is lg2? log base 2? *)
-(*     forall {w : nat} {nz : w <> O} (b1 b2 b3 : BitV w) t, *)
-(*       b3 = @lg2 w nz b1 b2 -> *)
-(*       eval_builtin ge lg2 (t :: (bits b1) :: (bits b2) :: nil) (bits b3) *)
-| eval_true :
-    eval_builtin ge true_builtin nil (bit true)
-| eval_false :
-    eval_builtin ge false_builtin nil (bit false)
-| eval_negate :
-    forall {w : nat} (b1 b2 : BitV w) t,
-      b2 = @neg w b1 ->
-      eval_builtin ge Neg (t :: (bits b1) :: nil) (bits b2)
-| eval_compl :
-    forall {w : nat} (b1 b2 : BitV w) t,
-      b2 = @not w b1 ->
-      eval_builtin ge Compl (t :: (bits b1) :: nil) (bits b2)
-| eval_lt :
-    forall {w : nat} (b1 b2 : BitV w) (b : bool) t,
-      b = @ltu w b1 b2 ->
-      eval_builtin ge Lt (t :: (bits b1) :: (bits b2) :: nil) (bit b)
-| eval_gt :
-    forall {w : nat} (b1 b2 : BitV w) (b : bool) t,
-      b = @gtu w b1 b2 ->
-      eval_builtin ge Gt (t :: (bits b1) :: (bits b2) :: nil) (bit b)
-| eval_le :  
-    forall {w : nat} (b1 b2 : BitV w) (b : bool) t,
-      b = @leu w b1 b2 ->
-      eval_builtin ge Le (t :: (bits b1) :: (bits b2) :: nil) (bit b)
-| eval_ge :
-    forall {w : nat} (b1 b2 : BitV w) (b : bool) t,
-      b = @geu w b1 b2 ->
-      eval_builtin ge Ge (t :: (bits b1) :: (bits b2) :: nil) (bit b)
-| eval_eq :
-    forall {w : nat} (b1 b2 : BitV w) (b : bool) t,
-      b = @eq w b1 b2 ->
-      eval_builtin ge Eq (t :: (bits b1) :: (bits b2) :: nil) (bit b)
-| eval_neq :
-    forall {w : nat} (b1 b2 : BitV w) (b : bool) t,
-      b = @neq w b1 b2 ->
-      eval_builtin ge Neq (t :: (bits b1) :: (bits b2) :: nil) (bit b)
-| eval_and :
-    forall {w : nat} (b1 b2 b3 : BitV w) t,
-      b3 = @and w b1 b2 ->
-      eval_builtin ge And (t :: (bits b1) :: (bits b2) :: nil) (bits b3)
-| eval_or :
-    forall {w : nat} (b1 b2 b3 : BitV w) t,
-      b3 = @or w b1 b2 ->
-      eval_builtin ge Or (t :: (bits b1) :: (bits b2) :: nil) (bits b3)
-| eval_xor :
-    forall {w : nat} (b1 b2 b3 : BitV w) t,
-      b3 = @xor w b1 b2 ->
-      eval_builtin ge Xor (t :: (bits b1) :: (bits b2) :: nil) (bits b3)
-| eval_zero : (* TODO: cryptol's builtin zero works in more cases than this *)
-    forall {ws : nat} (w : Z) (b : BitV ws),
-      ws = Z.to_nat w ->
-      b = @repr ws 0 -> 
-      eval_builtin ge Zero ((typ (TCon (TC (TCNum w)) nil)) :: nil) (bits b)
-| eval_shiftl :
-    forall {w : nat} (b1 b2 b3 : BitV w) t,
-      b3 = @shl w b1 b2 ->
-      eval_builtin ge Shiftl (t :: (bits b1) :: (bits b2) :: nil) (bits b3)
-| eval_shiftr :
-    forall {w : nat} (b1 b2 b3 : BitV w) t,
-      b3 = @shru w b1 b2 ->
-      eval_builtin ge Shiftr (t :: (bits b1) :: (bits b2) :: nil) (bits b3)
-| eval_rotl :    
-    forall {w : nat} (b1 b2 b3 : BitV w) t,
-      b3 = @rol w b1 b2 ->
-      eval_builtin ge Rotl (t :: (bits b1) :: (bits b2) :: nil) (bits b3)
-| eval_rotr :    
-    forall {w : nat} (b1 b2 b3 : BitV w) t,
-      b3 = @ror w b1 b2 ->
-      eval_builtin ge Rotr (t :: (bits b1) :: (bits b2) :: nil) (bits b3)
-(*| eval_append :
-    forall E t1 t2 t3 v1 v2 e1 e2,
-      e1 = EVar (1,"") ->
-      e2 = EVar (2,"") ->
-      E = extend (extend empty (1,"") v1) (2,"") v2  ->
-      eval_builtin ge Append (t1 :: t2 :: t3 :: v1 :: v2 :: nil) (* TODO *)*)
-| eval_at_bits :
-    forall {w : nat} E n e v t1 t2 t3 v1 (b : BitV w),
-      select_list ge E n e v ->
-      E = extend empty (0,"") v1 ->
-      e = EVar (0,"") ->
-      n = Z.to_nat (unsigned b) ->
-      eval_builtin ge At (t1 :: t2 :: t3 :: v1 :: (bits b) :: nil) v
-| eval_at_vnil : (* This case seems weird, but I think it's necessary *)
-    forall E e v t1 t2 t3 v1,
-      select_list ge E O e v ->
-      E = extend empty (0,"") v1 ->
-      e = EVar (0,"") ->
-      eval_builtin ge At (t1 :: t2 :: t3 :: v1 :: vnil :: nil) v
+    forall {w} (b1 b2 b3 : BitV w) E v1 v2 v3 l1 l2 t,
+      force_list ge E v1 l1 ->
+      force_list ge E v2 l2 ->
+      to_bitv l1 = Some b1 ->
+      to_bitv l2 = Some b2 ->
+      b3 = add b1 b2 ->
+      v3 = thunk_list (from_bitv b3) ->
+      eval_builtin ge E Plus (t :: v1 :: v2 :: nil) (v3)
+| eval_at_vnil : (* This case seems weird, but it's necessary (cryptol does this) *)
+    forall E l v t1 t2 t3 idx,
+      select_list ge E O l v ->
+      eval_expr ge E idx vnil ->
+      eval_builtin ge E At (t1 :: t2 :: t3 :: l :: idx :: nil) v
+(* | eval_minus : *)
+(*     forall {w : nat} (b1 b2 b3 : BitV w) t, *)
+(*       b3 = @sub w b1 b2 -> *)
+(*       eval_builtin ge Minus (t :: (bits b1) :: (bits b2) :: nil) (bits b3) *)
+(* | eval_times : *)
+(*     forall {w : nat} (b1 b2 b3 : BitV w) t, *)
+(*       b3 = @mul w b1 b2 -> *)
+(*       eval_builtin ge Times (t :: (bits b1) :: (bits b2) :: nil) (bits b3) *)
+(* | eval_div : *)
+(*     forall {w : nat} (b1 b2 b3 : BitV w) t, *)
+(*       b3 = @divu w b1 b2 -> (* I assume that division is unsigned in cryptol *) *)
+(*       unsigned b2 <> 0 -> (* no division by 0 *) *)
+(*       eval_builtin ge Div (t :: (bits b1) :: (bits b2) :: nil) (bits b3) *)
+(* | eval_mod : *)
+(*     forall {w : nat} (b1 b2 b3 : BitV w) t, *)
+(*       b3 = @modu w b1 b2 -> *)
+(*       eval_builtin ge Mod (t :: (bits b1) :: (bits b2) :: nil) (bits b3) *)
+(* (* | eval_exp : *) (* TODO: write pow over bits, or implement in Cryptol *) *)
+(* (*     forall {w : nat} {nz : w <> O} (b1 b2 b3 : BitV w) t, *) *)
+(* (*       b3 = @exp w nz b1 b2 -> *) *)
+(* (*       eval_builtin ge Exp (t :: (bits b1) :: (bits b2) :: nil) (bits b3) *) *)
+(* (* | eval_lg2 : *) (* TODO: what is lg2? log base 2? *) *)
+(* (*     forall {w : nat} {nz : w <> O} (b1 b2 b3 : BitV w) t, *) *)
+(* (*       b3 = @lg2 w nz b1 b2 -> *) *)
+(* (*       eval_builtin ge lg2 (t :: (bits b1) :: (bits b2) :: nil) (bits b3) *) *)
+(* | eval_true : *)
+(*     eval_builtin ge true_builtin nil (bit true) *)
+(* | eval_false : *)
+(*     eval_builtin ge false_builtin nil (bit false) *)
+(* | eval_negate : *)
+(*     forall {w : nat} (b1 b2 : BitV w) t, *)
+(*       b2 = @neg w b1 -> *)
+(*       eval_builtin ge Neg (t :: (bits b1) :: nil) (bits b2) *)
+(* | eval_compl : *)
+(*     forall {w : nat} (b1 b2 : BitV w) t, *)
+(*       b2 = @not w b1 -> *)
+(*       eval_builtin ge Compl (t :: (bits b1) :: nil) (bits b2) *)
+(* | eval_lt : *)
+(*     forall {w : nat} (b1 b2 : BitV w) (b : bool) t, *)
+(*       b = @ltu w b1 b2 -> *)
+(*       eval_builtin ge Lt (t :: (bits b1) :: (bits b2) :: nil) (bit b) *)
+(* | eval_gt : *)
+(*     forall {w : nat} (b1 b2 : BitV w) (b : bool) t, *)
+(*       b = @gtu w b1 b2 -> *)
+(*       eval_builtin ge Gt (t :: (bits b1) :: (bits b2) :: nil) (bit b) *)
+(* | eval_le :   *)
+(*     forall {w : nat} (b1 b2 : BitV w) (b : bool) t, *)
+(*       b = @leu w b1 b2 -> *)
+(*       eval_builtin ge Le (t :: (bits b1) :: (bits b2) :: nil) (bit b) *)
+(* | eval_ge : *)
+(*     forall {w : nat} (b1 b2 : BitV w) (b : bool) t, *)
+(*       b = @geu w b1 b2 -> *)
+(*       eval_builtin ge Ge (t :: (bits b1) :: (bits b2) :: nil) (bit b) *)
+(* | eval_eq : *)
+(*     forall {w : nat} (b1 b2 : BitV w) (b : bool) t, *)
+(*       b = @eq w b1 b2 -> *)
+(*       eval_builtin ge Eq (t :: (bits b1) :: (bits b2) :: nil) (bit b) *)
+(* | eval_neq : *)
+(*     forall {w : nat} (b1 b2 : BitV w) (b : bool) t, *)
+(*       b = @neq w b1 b2 -> *)
+(*       eval_builtin ge Neq (t :: (bits b1) :: (bits b2) :: nil) (bit b) *)
+(* | eval_and : *)
+(*     forall {w : nat} (b1 b2 b3 : BitV w) t, *)
+(*       b3 = @and w b1 b2 -> *)
+(*       eval_builtin ge And (t :: (bits b1) :: (bits b2) :: nil) (bits b3) *)
+(* | eval_or : *)
+(*     forall {w : nat} (b1 b2 b3 : BitV w) t, *)
+(*       b3 = @or w b1 b2 -> *)
+(*       eval_builtin ge Or (t :: (bits b1) :: (bits b2) :: nil) (bits b3) *)
+(* | eval_xor : *)
+(*     forall {w : nat} (b1 b2 b3 : BitV w) t, *)
+(*       b3 = @xor w b1 b2 -> *)
+(*       eval_builtin ge Xor (t :: (bits b1) :: (bits b2) :: nil) (bits b3) *)
+(* | eval_zero : (* TODO: cryptol's builtin zero works in more cases than this *) *)
+(*     forall {ws : nat} (w : Z) (b : BitV ws), *)
+(*       ws = Z.to_nat w -> *)
+(*       b = @repr ws 0 ->  *)
+(*       eval_builtin ge Zero ((typ (TCon (TC (TCNum w)) nil)) :: nil) (bits b) *)
+(* | eval_shiftl : *)
+(*     forall {w : nat} (b1 b2 b3 : BitV w) t, *)
+(*       b3 = @shl w b1 b2 -> *)
+(*       eval_builtin ge Shiftl (t :: (bits b1) :: (bits b2) :: nil) (bits b3) *)
+(* | eval_shiftr : *)
+(*     forall {w : nat} (b1 b2 b3 : BitV w) t, *)
+(*       b3 = @shru w b1 b2 -> *)
+(*       eval_builtin ge Shiftr (t :: (bits b1) :: (bits b2) :: nil) (bits b3) *)
+(* | eval_rotl :     *)
+(*     forall {w : nat} (b1 b2 b3 : BitV w) t, *)
+(*       b3 = @rol w b1 b2 -> *)
+(*       eval_builtin ge Rotl (t :: (bits b1) :: (bits b2) :: nil) (bits b3) *)
+(* | eval_rotr :     *)
+(*     forall {w : nat} (b1 b2 b3 : BitV w) t, *)
+(*       b3 = @ror w b1 b2 -> *)
+(*       eval_builtin ge Rotr (t :: (bits b1) :: (bits b2) :: nil) (bits b3) *)
+(* (*                    *)
+(* | eval_append : *)
+(*     forall E t1 t2 t3 v1 v2 e1 e2, *)
+(*       e1 = EVar (1,"") -> *)
+(*       e2 = EVar (2,"") -> *)
+(*       E = extend (extend empty (1,"") v1) (2,"") v2  -> *)
+(*       eval_expr ge E (EAppend e1 e2) v -> *)
+(*       eval_builtin ge Append (t1 :: t2 :: t3 :: v1 :: v2 :: nil) v *) *)
+(* | eval_at_bits : *)
+(*     forall {w : nat} E n e v t1 t2 t3 v1 (b : BitV w), *)
+(*       select_list ge E n e v -> *)
+(*       E = extend empty (0,"") v1 -> *)
+(*       e = EVar (0,"") -> *)
+(*       n = Z.to_nat (unsigned b) -> *)
+(*       eval_builtin ge At (t1 :: t2 :: t3 :: v1 :: (bits b) :: nil) v *)
 (*| eval_splitAt :
     forall E e v front back t,
       E = extend empty (1,"") v ->
